Add memory operations, at the cost of a few calls to magic/admit in the memory subsystem

src/arch/x64/X64.Machine_s.fst
@@ -9,6 +9,7 @@ unfold let nat128_max = Types_s.nat128_max
 unfold let nat64 = Types_s.nat64
 assume val int_to_nat64 : i:int -> n:nat64{0 <= i && i < nat64_max ==> i == n}
 unfold let nat128 = Types_s.nat128
+unfold let quad32 = Types_s.quad32
 
 type reg =
   | Rax
@@ -60,12 +61,17 @@ unfold let buffer8 = M.buffer (M.TBase M.TUInt8)
 unfold let buffer16 = M.buffer (M.TBase M.TUInt16)
 unfold let buffer32 = M.buffer (M.TBase M.TUInt32)
 unfold let buffer64 = M.buffer (M.TBase M.TUInt64)
+unfold let buffer128 = M.buffer (M.TBase M.TUInt128)
 assume val buffer_addr : #t:M.typ -> b:M.buffer t -> GTot int
 
 unfold let mem = M.mem
 assume val valid_mem64 : ptr:int -> h:mem -> bool // is there a 64-bit word at address ptr?
 assume val load_mem64 : ptr:int -> h:mem -> nat64 // the 64-bit word at ptr (if valid_mem64 holds)
 assume val store_mem64 : ptr:int -> v:nat64 -> h:mem -> mem
+
+assume val valid_mem128 (ptr:int) (h:mem) : bool
+assume val load_mem128  (ptr:int) (h:mem) : quad32 
+assume val store_mem128 (ptr:int) (v:quad32) (m:mem) : mem
 
 assume val lemma_valid_mem64 : b:buffer64 -> i:nat -> h:mem -> Lemma
   (requires
@@ -94,6 +100,33 @@ assume val lemma_store_mem64 : b:buffer64 -> i:int -> v:nat64 -> h:mem -> Lemma
     store_mem64 (buffer_addr b + 8 `op_Multiply` i) v h == M.buffer_write b i v h
   )
 
+assume val lemma_valid_mem128 : b:buffer128 -> i:nat -> h:mem -> Lemma
+  (requires
+    i < Seq.length (M.buffer_as_seq h b) /\
+    M.buffer_readable h b
+  )
+  (ensures
+    valid_mem128 (buffer_addr b + 16 `op_Multiply` i) h
+  )
+
+assume val lemma_load_mem128 : b:buffer128 -> i:int -> h:mem -> Lemma
+  (requires
+    i < Seq.length (M.buffer_as_seq h b) /\
+    M.buffer_readable h b
+  )
+  (ensures
+    load_mem128 (buffer_addr b + 16 `op_Multiply` i) h == M.buffer_read b i h
+  )
+
+assume val lemma_store_mem128 : b:buffer128 -> i:int -> v:quad32 -> h:mem -> Lemma
+  (requires
+    i < Seq.length (M.buffer_as_seq h b) /\
+    M.buffer_readable h b
+  )
+  (ensures
+    store_mem128 (buffer_addr b + 16 `op_Multiply` i) v h == M.buffer_write b i v h
+  )
+
 assume val lemma_store_load_mem64 : ptr:int -> v:nat64 -> h:mem -> Lemma
   (load_mem64 ptr (store_mem64 ptr v h) = v)
 
@@ -104,4 +137,14 @@ assume val lemma_frame_store_mem64: i:int -> v:nat64 -> h:mem -> Lemma (
 assume val lemma_valid_store_mem64: i:int -> v:nat64 -> h:mem -> Lemma (
   let h' = store_mem64 i v h in
   forall j. valid_mem64 j h <==> valid_mem64 j h')
- 
+
+assume val lemma_store_load_mem128 : ptr:int -> v:quad32 -> h:mem -> Lemma
+  (load_mem128 ptr (store_mem128 ptr v h) = v)
+
+assume val lemma_frame_store_mem128: i:int -> v:quad32 -> h:mem -> Lemma (
+  let h' = store_mem128 i v h in
+  forall i'. i' <> i /\ valid_mem128 i h /\ valid_mem128 i' h ==> load_mem128 i' h = load_mem128 i' h')
+
+assume val lemma_valid_store_mem128: i:int -> v:quad32 -> h:mem -> Lemma (
+  let h' = store_mem128 i v h in
+  forall j. valid_mem128 j h <==> valid_mem128 j h')
